src/SchemaWellFormedness.v
@@ -2,17 +2,21 @@ From mathcomp Require Import all_ssreflect.
 Set Implicit Arguments.
 Unset Strict Implicit.
 Unset Printing Implicit Defensive.
-From extructures Require Import ord fset.
+From extructures Require Import ord fset fmap.
+
+From Equations Require Import Equations.
 
 
 Require Import Schema.
 Require Import SchemaAux.
 
 
+
+
 Section WellFormedness.
 
   Variables (Name Vals : ordType).
-  Variable sch : @schema Name.
+  Implicit Type sch : @schema Name.
 
 
   
@@ -39,31 +43,31 @@ Section WellFormedness.
         be subtype of an interface and not between objects. Interfaces cannot be
         subtype of another interface.
    **)
-  Inductive Subtype : type -> type -> Prop :=
-  | ST_Refl : forall ty, Subtype ty ty
+  Inductive Subtype sch : type -> type -> Prop :=
+  | ST_Refl : forall ty, Subtype sch ty ty
                             
   | ST_Interface : forall n n',
       declares_implementation sch n n' ->
-      Subtype (NT n) (NT n')
+      Subtype sch (NT n) (NT n')
               
   | ST_Union : forall n n',
       (n \in (union_members sch n')) ->
-      Subtype (NT n) (NT n')
+      Subtype sch (NT n) (NT n')
                     
   | ST_ListType : forall ty ty',
-      Subtype ty ty' ->
-      Subtype (ListType ty) (ListType ty'). 
+      Subtype sch ty ty' ->
+      Subtype sch (ListType ty) (ListType ty'). 
 
-  Fixpoint is_subtype (ty ty' : type) : bool :=
+  Fixpoint is_subtype sch (ty ty' : type) : bool :=
     match ty, ty' with
-    | (ListType lty), (ListType lty') => is_subtype lty lty'
+    | (ListType lty), (ListType lty') => is_subtype sch lty lty'
     | (NT name), (NT name') => [|| (name == name'),
                                declares_implementation sch ty ty' | 
                               (name \in (union_members sch name'))]
     | _, _ => false
     end.
 
-   Lemma subtypeP ty ty': reflect (Subtype ty ty') (is_subtype ty ty').
+   Lemma subtypeP sch ty ty': reflect (Subtype sch ty ty') (is_subtype sch ty ty').
    Proof.
     apply: (iffP idP).
     elim: ty ty' => n.
@@ -87,25 +91,25 @@ Section WellFormedness.
 
       https://facebook.github.io/graphql/June2018/#sec-Input-and-Output-Types **)
 
-  Inductive valid_argument_type : type -> Prop :=
+  Inductive valid_argument_type sch : type -> Prop :=
   | VScalar_Arg : forall ty,
       is_scalar_type sch ty ->
-      valid_argument_type (NT ty)
+      valid_argument_type sch (NT ty)
   | VEnum_Arg : forall ty,
       is_enum_type sch ty ->
-      valid_argument_type (NT ty)
+      valid_argument_type sch (NT ty)
   | VList_Arg : forall ty,
-      valid_argument_type ty ->
-      valid_argument_type (ListType ty).
+      valid_argument_type sch ty ->
+      valid_argument_type sch (ListType ty).
   
-  Fixpoint is_valid_argument_type (ty : type) : bool :=
+  Fixpoint is_valid_argument_type sch (ty : type) : bool :=
     match ty with
     | NT name => is_scalar_type sch ty || is_enum_type sch ty
-    | ListType ty' => is_valid_argument_type ty'
+    | ListType ty' => is_valid_argument_type sch ty'
     end.
 
 
-  Lemma valid_argument_typeP : forall ty, reflect (valid_argument_type ty) (is_valid_argument_type ty).
+  Lemma valid_argument_typeP sch : forall ty, reflect (valid_argument_type sch ty) (is_valid_argument_type sch ty).
   Proof.
     move=> ty; apply: (iffP idP).
     elim: ty.
@@ -118,22 +122,22 @@ Section WellFormedness.
   
   (* Because we are not considering InputObjects, a field may have any type, 
      as long as it is declared in the Schema. *)
-  Inductive valid_field_type : type -> Prop :=
+  Inductive valid_field_type sch : type -> Prop :=
   | VBase_Type : forall n,
       is_declared sch n ->
-      valid_field_type (NT n)      
+      valid_field_type sch (NT n)      
   | VList_Type : forall ty,
-      valid_field_type ty ->
-      valid_field_type (ListType ty).
+      valid_field_type sch ty ->
+      valid_field_type sch (ListType ty).
   
-  Fixpoint is_valid_field_type (ty : type) : bool :=
+  Fixpoint is_valid_field_type sch (ty : type) : bool :=
     match ty with
     | NT n => is_declared sch n
-    | ListType ty' => is_valid_field_type ty'
+    | ListType ty' => is_valid_field_type sch ty'
     end.
   
 
-  Lemma valid_field_typeP : forall ty, reflect (valid_field_type ty) (is_valid_field_type ty).
+  Lemma valid_field_typeP sch : forall ty, reflect (valid_field_type sch ty) (is_valid_field_type sch ty).
   Proof.
     move=> ty; apply: (iffP idP); last by elim.
     elim: ty.
@@ -145,8 +149,8 @@ Section WellFormedness.
   (** 
       It checks whether an argument is well-formed by checking that
       its type is a valid type for an argument **)
-  Definition is_field_argument_wf (arg : FieldArgumentDefinition) : bool :=
-    is_valid_argument_type arg.(argtype).
+  Definition is_field_argument_wf sch (arg : FieldArgumentDefinition) : bool :=
+    is_valid_argument_type sch arg.(argtype).
 
   
   (**
@@ -158,36 +162,26 @@ Section WellFormedness.
            ------------------------------
            (fname (args) : ty) isAWellFormedField
    **)
-  Definition is_field_wf (fld : FieldDefinition) : bool :=
-    [&& is_valid_field_type fld.(return_type),
-     uniq [seq arg.(argname) | arg <- fld.(fargs)] &
-     all (is_field_argument_wf) fld.(fargs)].
+  Definition is_field_wf sch (fld : FieldDefinition) : bool :=
+    is_valid_field_type sch fld.(return_type) &&
+     (* uniq [seq arg.(argname) | arg <- fld.(fargs)] &  // Not specified... But should be? *)
+     all (is_field_argument_wf sch) fld.(fargs).
 
 
 
   (** This checks whether an object field is valid w/r to another from an implemented interface.
-      The possible options are:
+      It checks the following:
+      1. Both fields have the same name.
+      2. The arguments of the interface field must be a subset of the object's arguments.
+      3. The object's field return type must be a subtype of the interface's field.
 
-
-    3.      T <: U     ∀ arg ∈ args', arg ∈ args          
-            -------------------------------------------
-             (fname (args) : T) OK (fname (args') : U)
-
-    4.      T ∈ unionTypes(U)     ∀ arg ∈ args', arg ∈ args
-           --------------------------------------------------------
-                 (fname (args) : T) OK (fname (args') : U)
-
-
-    The arguments have to be completed included, both their names and types (invariant).
-
+      This is not checking that any additional argument in the object must be a "non-required" field.
    **)
-  Definition is_field_ok (fld fld' : FieldDefinition) : bool :=
-    match fld, fld' with
-    | Field fname args ty, Field fname' args' ty' =>
-      [&& (fname == fname'),
-       fsubset args' args &
-       is_subtype ty ty']
-    end.
+  Definition is_field_ok sch (fld fld' : FieldDefinition) : bool :=
+    [&& (fld.(fname) == fld'.(fname)),
+     fsubset fld'.(fargs) fld.(fargs) &
+     is_subtype sch fld.(return_type) fld'.(return_type)].
+    
 
 
 
@@ -215,12 +209,27 @@ Section WellFormedness.
       implementsOK schema (NamedType name) (NamedType iname).
 
 *)
-  Definition implements_interface_correctly (ty ty' : NamedType) : bool :=
+  Definition implements_interface_correctly sch (ty ty' : NamedType) : bool :=
     let ifields := fields sch ty' in
     let ofields := fields sch ty in
-    all (fun f' => has (fun f => is_field_ok f f') ofields) ifields.
+    all (fun f' => has (fun f => is_field_ok sch f f') ofields) ifields.
      
 
+  Lemma implements_interface_correctlyP sch (ity ty : NamedType) :
+    reflect (forall fi, fi \in fields sch ity ->
+                          exists f, f \in fields sch ty /\ is_field_ok sch f fi)
+            (implements_interface_correctly sch ty ity).
+  Proof.
+    apply: (iffP idP).
+    - rewrite /implements_interface_correctly => /allP H.
+      by move=> fi /H /hasP [f Hin Hok]; exists f.
+    - move=> H.
+      rewrite /implements_interface_correctly.
+      apply/allP => fi Hin.
+      apply/hasP.
+      by move: (H fi Hin) => [f [Hin' Hok]]; exists f.
+  Qed.
+  
   (**
 
                        Schema(S) = scalar S 
@@ -262,47 +271,23 @@ Section WellFormedness.
                           enum E { Evs } 
 
    **)
-  (*
-  Inductive wf_type_definition : TypeDefinition -> Prop :=
-  | WF_Scalar : forall name, wf_type_definition (ScalarTypeDefinition name)
-                       
-  | WF_Object : forall name (interfaces : {fset NamedType}) fields,
-      fields != [::] ->
-      uniq [seq fld.(field_name) | fld <- fields] ->
-      all is_field_wf fields ->
-      all (implements_interface_correctly name) interfaces ->
-      wf_type_definition (ObjectTypeDefinition name interfaces fields)
-                       
-  | WF_Interface : forall name fields,
-      fields != [::] ->
-      uniq [seq fld.(field_name) | fld <- fields] ->
-      all is_field_wf fields ->
-      wf_type_definition (InterfaceTypeDefinition name fields)
-                       
-  | WF_Union : forall name (members : {fset NamedType}),
-      members != fset0 ->
-      all (is_object_type schema) members ->
-      wf_type_definition (UnionTypeDefinition name members)
-                       
-  | WF_Enum : forall name enumValues,
-      enumValues != fset0 ->
-      wf_type_definition (EnumTypeDefinition name enumValues).
-   *)
+  
 
-  Fixpoint is_type_def_wf (tdef : TypeDefinition) : bool :=
+  Fixpoint is_type_def_wf sch (tdef : TypeDefinition) : bool :=
     match tdef with
     | ScalarTypeDefinition _ => true
                                  
     | ObjectTypeDefinition name interfaces fields =>
       [&& (fields != [::]),
        uniq [seq fld.(fname) | fld <- fields],
-       all is_field_wf fields &
-       all (implements_interface_correctly name) interfaces]
+       all (is_field_wf sch) fields,
+       all (is_interface_type sch) interfaces &
+       all (implements_interface_correctly sch name) interfaces]
 
     | InterfaceTypeDefinition _ fields =>
       [&& (fields != [::]),
        uniq [seq fld.(fname) | fld <- fields] &
-       all is_field_wf fields]
+       all (is_field_wf sch) fields]
 
     | UnionTypeDefinition name members =>
       (members != fset0) && all (is_object_type sch) members
@@ -312,22 +297,37 @@ Section WellFormedness.
     end.
 
 
+  Lemma is_type_def_wf_objE sch name interfaces fields :
+    is_type_def_wf sch (ObjectTypeDefinition name interfaces fields) =
+    [&& (fields != [::]),
+       uniq [seq fld.(fname) | fld <- fields],
+       all (is_field_wf sch) fields,
+       all (is_interface_type sch) interfaces &
+       all (implements_interface_correctly sch name) interfaces].
+  Proof.
+      by case: sch. Qed.
+
+  Lemma is_type_def_wf_unionE sch name mbs :
+    is_type_def_wf sch (UnionTypeDefinition name mbs) = (mbs != fset0) && all (is_object_type sch) mbs.
+  Proof. by case: sch. Qed.
+
+    
   
-  Definition is_schema_wf schema : bool :=
-    [&& (schema.(query_type) \in schema_names schema),
-     is_object_type schema schema.(query_type),
-     uniq [seq tdef.(tdname) | tdef <- schema] &                   
-     all is_type_def_wf schema.(type_definitions)].
+  Definition is_schema_wf sch : bool :=
+    [&& (sch.(query_type) \in schema_names sch),
+     is_object_type sch sch.(query_type),
+     all (fun p => has_name p.1 p.2) sch.(type_definitions) &
+     all (fun p => is_type_def_wf sch p.2) sch.(type_definitions)].
       
   
   Structure wfSchema := WFSchema {
-                        schem : @schema Name;
-                        hasType :  Name -> Vals -> bool;
-                        _ : is_schema_wf schem;
+                           sch;
+                           hasType :  Name -> Vals -> bool;
+                           _ : is_schema_wf sch;
                       }.
 
   
-  Coercion schem : wfSchema >-> Schema.schema.
+  Coercion sch : wfSchema >-> Schema.schema.
 
 
 
@@ -348,26 +348,208 @@ Section WellFormedness.
 
   Lemma tdefs_N_nil schema :
     is_schema_wf schema ->
-    schema.(type_definitions) != [::].
+    schema.(type_definitions) != emptym.
   Proof.
     rewrite /is_schema_wf => /and4P [H _ _ _].
     rewrite /schema_names in_fset in H.
-    by case: schema.(type_definitions) H => //.
+    move/mapP: H => [x /codommP [t Hs] H].
+    case: (type_definitions schema) Hs.
+    by case.
+  Qed.
+
+  Lemma lookup_type_name_wf schema ty tdef :
+    is_schema_wf schema ->
+    lookup_type schema ty = Some tdef ->
+    ty = tdef.(tdname).
+  Proof.
+    rewrite /is_schema_wf => /and4P [_ _ /allP H _].
+    rewrite /lookup_type.
+    move/getmP=> Hin.
+    by move/has_nameP: (H (ty, tdef) Hin) => /=.
   Qed.
 
   
-  Lemma has_implementation_is_interface (schema : wfSchema) ty :
+
+
+  Lemma lookup_in_schema_wfP schema ty tdef :
+    is_schema_wf schema ->
+    reflect (lookup_type schema ty = Some tdef /\ ty = tdef.(tdname))
+            ((ty, tdef) \in schema.(type_definitions)).
+  Proof.
+    move=> Hwf.
+    apply: (iffP idP).
+    - move: Hwf; rewrite /is_schema_wf => /and4P [_ _ /allP H _].
+      move=> Hin.
+      move/has_nameP: (H (ty, tdef) Hin) => /= Heq.
+      rewrite Heq in Hin *.
+        by move/lookup_in_schemaP: Hin; split.
+    - move=> [Hlook Heq].
+      by apply/lookup_in_schemaP.
+  Qed.
+
+ 
+  Lemma is_scalar_type_wfE schema ty :
+    is_schema_wf schema ->
+    reflect (lookup_type schema ty = Some (ScalarTypeDefinition ty))
+            (is_scalar_type schema ty).
+  Proof.
+    move=> Hwf.
+    apply: (iffP idP).
+    - rewrite /is_scalar_type.
+      case Hlook: lookup_type => [tdef|] //.
+      move: (lookup_type_name_wf Hwf Hlook) => ->.
+        by case: tdef {Hlook}.
+    - move=> Hlook.
+      by rewrite /is_scalar_type Hlook.
+  Qed.
+
+  Lemma is_object_type_wfP schema ty :
+    is_schema_wf schema ->
+    reflect (exists intfs flds, lookup_type schema ty = Some (ObjectTypeDefinition ty intfs flds))
+            (is_object_type schema ty).
+  Proof.
+    move=> Hwf.
+    apply: (iffP idP)=> //.
+    - funelim (is_object_type schema ty) => // _.
+      exists f, l; move: (lookup_type_name_wf Hwf Heq) => H.
+        by rewrite H in Heq * => /=.
+    - move=> [intfs [flds Hlook]].
+        by rewrite /is_object_type Hlook.
+  Qed.
+
+  Lemma is_interface_type_wfP schema ty :
+    is_schema_wf schema ->
+    reflect (exists flds, lookup_type schema ty = Some (InterfaceTypeDefinition ty flds))
+            (is_interface_type schema ty).
+  Proof.
+    move=> Hwf.
+    apply: (iffP idP).
+    - funelim (is_interface_type schema ty) => // _.
+      exists l0; move: (lookup_type_name_wf Hwf Heq) => H.
+        by rewrite H in Heq *.
+    - move=> [flds Hlook].
+      by rewrite /is_interface_type Hlook.
+  Qed.
+ 
+
+  Lemma is_union_type_wfP schema ty :
+    is_schema_wf schema ->
+    reflect (exists mbs, lookup_type schema ty = Some (UnionTypeDefinition ty mbs))
+            (is_union_type schema ty).
+  Proof.
+    move=> Hwf.
+    apply: (iffP idP).
+    - funelim (is_union_type schema ty) => // _.
+      exists f0; move: (lookup_type_name_wf Hwf Heq) => H.
+        by rewrite H in Heq *.
+    - move=> [mbs Hlook].
+      by rewrite /is_union_type Hlook.
+  Qed.
+
+      
+  Lemma implements_declares_implementation schema (ity : Name) (tdef : TypeDefinition) :
+    is_schema_wf schema ->
+    (tdef.(tdname), tdef) \in schema.(type_definitions) ->
+    declares_implementation schema tdef.(tdname) ity <-> implements_interface ity tdef.
+  Proof.
+    move=> Hwf.
+    move/lookup_in_schemaP=> Htdef.
+    split.
+    - rewrite /declares_implementation.
+      rewrite Htdef.
+      case: tdef Htdef => // o i f Hin.
+    - rewrite /implements_interface /declares_implementation Htdef.
+      by case: tdef Htdef.
+  Qed.
+    
+  Lemma declares_implementation_are_interfaces schema tdef (ity : Name) :
+    is_schema_wf schema ->
+    declares_implementation schema tdef ity ->
+    is_interface_type schema ity.
+  Proof.
+    move=> Hwf Hdecl.
+    move: (declares_implementation_is_object Hdecl).
+    move/(is_object_type_wfP tdef Hwf) => [intfs [flds /lookup_in_schemaP Hlook]].
+    move/and4P: Hwf => [_ _ _ /allP Hok].
+    move: (Hok (tdef, ObjectTypeDefinition tdef intfs flds) Hlook).
+    rewrite is_type_def_wf_objE => /and5P [_ _ _ /allP Hintf _].
+    rewrite /declares_implementation in Hdecl.
+    move/lookup_in_schemaP: Hlook => Hlook.
+    rewrite Hlook in Hdecl.
+    apply (Hintf ity Hdecl).
+  Qed.    
+    
+    
+  Lemma has_implementation_is_interface schema ty :
+    is_schema_wf schema ->
     implementation schema ty != fset0 ->
     is_interface_type schema ty.
   Proof.
-  Abort.
-  
-  Lemma field_in_interface_in_object (schema : wfSchema) ty ti f :
+    move=> Hwf.
+    move/implementationP=> [tdef /codommP [t  Hlook]].
+    move: (lookup_type_name_wf Hwf Hlook) => Heq; rewrite Heq in Hlook.
+    move/lookup_in_schemaP: Hlook => Hin.
+    move/(implements_declares_implementation ty Hwf Hin).
+    by apply: declares_implementation_are_interfaces.
+  Qed.
+
+ 
+    
+  Lemma field_in_interface_in_object schema ty ti f :
+    is_schema_wf schema ->
     ty \in implementation schema ti ->
-    lookup_field_in_type schema ty f = lookup_field_in_type schema ti f.
+    lookup_field_in_type schema ti f -> lookup_field_in_type schema ty f.
   Proof.
-    Admitted.
-           
+    move=> Hwf Hin.
+    move/declares_in_implementation: Hin => Hdecl.
+    move: (declares_implementation_is_object Hdecl) => /(is_object_type_wfP ty Hwf).
+    case=> [intfs [flds Hlook]].
+    rewrite {2}/lookup_field_in_type Hlook.
+    move/lookup_field_in_typeP=> [tdef [ty' [Hlook' Hfin]]] Heq /=.
+    move: (lookup_type_name_wf Hwf Hlook') => Heq'.
+    rewrite /declares_implementation Hlook in Hdecl.
+    move: (lookup_type_name_wf Hwf Hlook) => Hneq.
+
+    move/lookup_in_schemaP: Hlook => Hin.
+    move/and4P: Hwf => [_ _ _ /allP Hok].
+    move: (Hok (ty, (ObjectTypeDefinition ty intfs flds)) Hin) => {Hok}.
+    rewrite is_type_def_wf_objE => /and5P [_ _ _ _ /allP Hintfs].
+    move: (Hintfs ti Hdecl) => {Hintfs Hdecl}.
+    move/implements_interface_correctlyP => H'.
+    move/lookup_in_schemaP: Hlook'.
+    rewrite Heq' => Hin'.
+    move: Hfin.
+    rewrite -(fields_E Hin') => Hfields.
+    rewrite -Heq' in Hfields.
+    move: (H' ty' Hfields) => [fld [Hfin Hok]].
+    apply/get_firstP.
+    exists fld.
+    rewrite Hneq in Hin.
+      by rewrite (fields_E Hin) in Hfin => /=.
+      apply/has_field_nameP.
+      move: Hok; rewrite /is_field_ok => [/and3P [/eqP HE]] _ _.
+      by rewrite -Heq.
+  Qed.
+
+
+  Lemma union_members_nfset0Pwf schema ty :
+    is_schema_wf schema ->
+    reflect (is_union_type schema ty) (union_members schema ty != fset0).
+  Proof.
+    move=> Hwf.
+    apply: (iffP idP).
+    - move/fset0Pn=> [x].
+      rewrite /union_members.
+      funelim (is_union_type schema ty) => //; rewrite Heq //.
+    - funelim (is_union_type schema ty) => // _.
+      rewrite /union_members Heq.
+      move/lookup_in_schemaP: Heq.
+      move/and4P: Hwf => [_ _ _ /allP Hok].
+      move/(Hok (ty, UnionTypeDefinition s2 f0)) => /=.
+      by rewrite is_type_def_wf_unionE => /andP [H _].
+  Qed.
+  
+  
 End WellFormedness.
 
 
